galois/network/action.lean
@@ -1,0 +1,129 @@
+import galois.map.fmap_func
+       galois.network.labels
+
+universes u v
+
+
+namespace network
+
+inductive act (A : Type u) : Type u
+| return : A → act
+| connect : remote_name → (socket → act) → act
+| send_message : socket -> message_t → act → act
+-- return a poll result and the amount of time elapsed
+| poll : Π (ports : list port) (sockets : list socket) (bound : time), 
+     (poll_result ports sockets bound → act) → act
+
+def act_bind {A B : Type u} (x : act A) (f : A → act B) : act B
+:= begin
+induction x,
+{ apply f, assumption },
+{ apply act.connect; assumption },
+{ apply act.send_message; assumption },
+{ apply act.poll; try {assumption} }
+end
+
+lemma act_bind_pure {α : Type u} (x : act α)
+: act_bind x act.return = x :=
+begin
+  simp [act_bind], induction x; dsimp,
+  { reflexivity },
+  { dsimp at ih_1,  
+    apply congr_arg, apply funext,
+    intros s, apply ih_1 },
+  { apply congr_arg, apply ih_1 },
+  { dsimp at ih_1,
+    apply congr_arg, apply funext,
+    intros t, apply ih_1 }
+end
+
+instance act_is_monad : monad act :=
+{ pure := @act.return
+, bind := @act_bind
+, id_map := begin intros, dsimp, apply act_bind_pure end
+, pure_bind :=
+begin
+  intros, simp [act_bind],
+end
+, bind_assoc :=
+begin
+  intros, induction x,
+  { reflexivity },
+  { simp [act_bind], dsimp,
+    apply congr_arg, apply funext,
+    intros s, apply ih_1 },
+  { simp [act_bind],
+    apply congr_arg, apply ih_1 },
+  { simp [act_bind], dsimp,
+    apply congr_arg, apply funext,
+    intros s, apply ih_1 }
+end
+}
+
+instance act_is_network_monad : network_monad act :=
+  { to_monad := network.act_is_monad
+  , socket := remote_name
+  , connect := λ x, act.connect x act.return
+  , send := λ x y, act.send_message x y (act.return punit.star)
+  , poll := λ x y z, act.poll x y z act.return  
+  }
+
+lemma act_bind_poll {A : Type} {ports sockets bound}
+  (f : poll_result ports sockets bound → act A)
+  : poll ports sockets bound >>= f
+  = act.poll ports sockets bound f
+:= rfl
+
+lemma act_bind_send {B : Type} {rn : remote_name}
+  {mess : message_t}
+  (f : act B)
+  : @send _ network.act_is_network_monad rn mess >> f 
+    = act.send_message rn mess f
+  := rfl
+
+lemma act_bind_connect {B : Type} {rn : remote_name}
+  (f : socket → act B)
+  : @network_monad.connect _ network.act_is_network_monad rn >>= f 
+    = act.connect rn f
+  := rfl
+
+lemma act_bind_return {A B : Type} {x : A}
+  (f : A → act B)
+  : return x >>= f 
+    = f x
+  := rfl
+    
+
+-- An agent is defined as a type for the internal state, an process that produces
+-- the state, and a looping process that will execute when the process is complete.
+--
+-- Semantically, think of the behavior as `next >>= forever loop` where
+-- `forever loop = loop >=> forever loop`.
+structure agent : Type 1 :=
+  (state_type : Type)
+  (loop : state_type → act state_type)
+
+
+section
+parameters (ag : agent)
+
+parameter {poll_receive_label_impl : list port → list socket → Type}
+
+inductive poll_dlabel (ports : list port) (sockets : list socket) (bound : ℕ) : Type
+| timeout {} : poll_dlabel
+| receive {} : ∀ (elapsed_fin : fin bound) (rn : remote_name),
+    poll_receive_label_impl ports sockets
+    → poll_dlabel
+
+inductive dlabel : act ag.state_type → Type
+| update_own_state : ∀ new_state : ag.state_type, dlabel (act.return new_state)
+| connect : ∀ (rn : remote_name) cont, dlabel (act.connect rn cont)
+| send_message : ∀ sock mess cont,
+      dlabel (act.send_message sock mess cont)
+| poll : ∀ (ports : list port) (sockets : list socket) (bound : time) cont,
+    poll_dlabel ports sockets bound
+    → dlabel (act.poll ports sockets bound cont)
+
+end
+
+end network
