galois/network/network_local_abs.lean
@@ -1,0 +1,71 @@
+/-
+For a given agent, we define a labeled transition system
+where everything else occuring on the network may be completely arbitrary
+-/
+import .action
+
+namespace network
+namespace loc
+
+inductive poll_receive_dlabel_abs (ports : list port) (sockets : list socket)
+    : Type
+| new_connection {} : ports.member → socket → poll_receive_dlabel_abs
+| receive_message {} : sockets.member → message_t → poll_receive_dlabel_abs
+
+@[reducible]
+def dlabel' {a} := @dlabel a poll_receive_dlabel_abs
+
+section
+parameters (a_ip : ip) (ag : agent)
+
+def next_receive_dlabel {ports : list port} {sockets : list socket}
+  {bound : time}
+  (cont : poll_result ports sockets bound → act ag.state_type)
+  (elapsed_fin : fin bound) (rn : remote_name)
+  : poll_receive_dlabel_abs ports sockets
+  → act ag.state_type
+| (poll_receive_dlabel_abs.new_connection p sock) :=
+     cont (poll_result.new_connection elapsed_fin p sock)
+| (poll_receive_dlabel_abs.receive_message sock mess) := 
+     cont (poll_result.message elapsed_fin sock mess)
+
+def next_poll_dlabel {ports : list port} {sockets : list socket}
+  {bound : time} (cont : poll_result ports sockets bound → act ag.state_type)
+  : @poll_dlabel poll_receive_dlabel_abs ports sockets bound 
+  → act ag.state_type
+| poll_dlabel.timeout := cont poll_result.timeout
+| (poll_dlabel.receive elapsed_fin rn rlabel) := next_receive_dlabel
+     cont elapsed_fin rn rlabel
+
+def next_agent_state_from_dlabel
+  : ∀ (a_next : act ag.state_type) (la : dlabel' a_next)
+  , act ag.state_type
+| (act.return new_state) (dlabel.update_own_state ._) := ag.loop new_state
+| (act.connect rn cont) (dlabel.connect ._ ._) := cont rn
+| (act.send_message sock mess cont) (dlabel.send_message ._ ._ ._) := cont
+| (act.poll ports sockets bound cont) (dlabel.poll ._ ._ ._ ._ plabel)
+    := next_poll_dlabel cont plabel
+
+inductive sends_message_st (P : socket → message_t → Prop) : act ag.state_type → Prop
+| mk : ∀ sock mess cont, P sock mess 
+     → sends_message_st (act.send_message sock mess cont)
+
+instance sends_message_st_decidable (P : socket → message_t → Prop) 
+  [decP : ∀ x y, decidable (P x y)] : decidable_pred (sends_message_st P)
+:= begin
+intros x, induction x;
+  try { solve1 {apply decidable.is_false, intros x, cases x} },
+have H := decP a a_1, induction H,
+{ apply decidable.is_false, intros contra, cases contra,
+  apply a_3, assumption },
+{ apply decidable.is_true, 
+  constructor, assumption
+}
+end
+
+def LTS s l s' := next_agent_state_from_dlabel s l = s'
+
+end
+
+end loc
+end network
